Intermediate/GlobalEnv.v
@@ -27,7 +27,8 @@ Definition executing G (pc : Pointer.t) (i : instr) : Prop :=
   exists C_procs P_code,
     NMap.find (Pointer.component pc) (genv_procedures G) = Some C_procs /\
     NMap.find (Pointer.block pc) C_procs = Some P_code /\
-    nth_error P_code (Pointer.offset pc) = Some i.
+    (Pointer.offset pc >= 0)%Z /\
+    nth_error P_code (Z.to_nat (Pointer.offset pc)) = Some i.
 
 Fixpoint find_label (c : code) (l : label) : option nat :=
   let fix aux c o :=
@@ -49,7 +50,7 @@ Definition find_label_in_procedure G (pc : Pointer.t) (l : label) : option Point
     match NMap.find (Pointer.block pc) C_procs with
     | Some P_code =>
       match find_label P_code l with
-      | Some offset => Some (Pointer.component pc, Pointer.block pc, offset)
+      | Some offset => Some (Pointer.component pc, Pointer.block pc, Z.of_nat offset)
       | None => None
       end
     | None => None
@@ -64,7 +65,7 @@ Definition find_label_in_component G (pc : Pointer.t) (l : label) : option Point
         match ps with
         | [] => None
         | (p_block,p_code) :: ps' =>
-          match find_label_in_procedure G (Pointer.component pc, p_block, 0) l with
+          match find_label_in_procedure G (Pointer.component pc, p_block, 0%Z) l with
           | None => search ps'
           | Some ptr => Some ptr
           end
